Workbench.v
@@ -4,349 +4,180 @@ Import SnoclistNotations.
 Require Import PlanarLambda.
 Require Import Types.
 
+Require Import Subst.
+Require Import LabeledLambda.
+Require Import Bidir.
+
 Require Import Coq.Program.Equality.
+Require Import Coq.Sorting.Permutation.
 Require Import Arith.
 Require List.
 
-Definition context n : Type := snoclist type n.
-
-Inductive is_typed : forall {a : nat}, context a -> pterm a -> type -> Prop :=
-| typed_var ty : is_typed [ty] PVar ty
-| typed_abs {n} ty1 gamma (pt : pterm (S n)) ty2 :
-  is_typed (gamma :: ty1) pt ty2 -> is_typed gamma (PAbs pt) (TImp ty1 ty2)
-| typed_app {n m} gamma delta (pt1 : pterm n) (pt2 : pterm m) ty1 ty2:
-  is_typed gamma pt1 (TImp ty1 ty2) -> is_typed delta pt2 ty1 ->
-  is_typed (gamma ++ delta) (PApp pt1 pt2) ty2.
-
-(* ===== Substitution ===== *)
-
-Definition s_rule : Type := nat * type.
-Definition s_rules : Type := list s_rule.
-
-Fixpoint subst1_ty (rul : s_rule) (ty : type) : type :=
-match ty with
-| TVar n => let (m, u) := rul in
-  match eqb n m with
-  | true => u
-  | false => ty
-  end
-| TImp ty1 ty2 => TImp (subst1_ty rul ty1) (subst1_ty rul ty2)
-end.
-
-Fixpoint subst_ty (sigma : s_rules) (ty : type) : type :=
-match sigma with
-| List.nil => ty
-| List.cons rul sigma' =>
-  subst_ty sigma' (subst1_ty rul ty)
-end.
-
-Fixpoint subst1_ctx {n : nat} (rul : s_rule) (ctx : context n) : context n :=
-match ctx with
-| [] => []
-| ctx' :: ty => (subst1_ctx rul ctx') :: (subst1_ty rul ty)
-end.
-
-Fixpoint subst_ctx {n : nat} (sigma : s_rules) (ctx : context n) : context n :=
-match sigma with
-| List.nil => ctx
-| List.cons rul sigma' =>
-  subst_ctx sigma' (subst1_ctx rul ctx)
-end.
-
-Axiom comm_nil : forall (A : Type), snoclist_comm [] (A := A) (m := 0) (n := 0) = [].
-
-Axiom comm_appnil : forall (A : Type) (n : nat) (l : snoclist A n) (a : A),
-  snoclist_comm (l :: a) (m := 0) (n := S n) = snoclist_comm l (m := 0) (n := n) :: a.
-
-Axiom comm_nilapp : forall (A : Type) (n : nat) (l : snoclist A n) (a : A),
-  snoclist_comm (snoclist_comm ([] ++ l) :: a) (m := S n) (n := 0) = l :: a.
-
-Theorem snoclist_asso_1 {A : Type} {n m : nat} : snoclist A (S m + n) -> snoclist A (m + S n).
-Proof. rewrite Nat.add_succ_comm. intro h. apply h. Qed.
-
-Axiom comm_consapp_asso : forall (A : Type) (m n : nat) (l : snoclist A m) (r : snoclist A n) (a : A),
-  snoclist_comm (snoclist_comm (l ++ r) (m := m) (n := n) :: a) (m := S n) (n := m) =
-  snoclist_asso_1 ((l ++ r) :: a).
-
-Axiom comm_consapp_asso' : forall (A : Type) (m n : nat) (l : snoclist A m) (r : snoclist A n) (a b : A),
-  snoclist_comm (snoclist_comm ((l :: a) ++ r) (m := S m) (n := n) :: b) (m := S n) (n := S m) =
-  snoclist_asso_1 ((l :: a) ++ r) :: b.
-
-Axiom P_asso : forall {A : Type} (m n : nat) (l : snoclist A (S m + n))
-  (P : forall {n : nat}, snoclist A n -> snoclist A n),
-  P (snoclist_asso_1 l) = snoclist_asso_1 (P l).
-
-Axiom P_comm : forall {A : Type} (m n : nat) (l : snoclist A (m + n))
-  (P : forall {n : nat}, snoclist A n -> snoclist A n),
-  P (snoclist_comm l) = snoclist_comm (P l).
-
-Lemma subst_asso : forall {m n : nat} (rul : s_rule) (ctx : context (S m + n)),
-  subst1_ctx rul (snoclist_asso_1 ctx) = 
-  snoclist_asso_1 (subst1_ctx rul ctx).
-Proof. intros m n rul ctx. Admitted.
-(* apply P_asso with (m := m) (n := n) (l := ctx) (P := subst1_ctx rul). *)
-
-Axiom asso_eq : forall {m n : nat} (ctx1 ctx2 : context (S m + n)),
-  snoclist_asso_1 ctx1 = snoclist_asso_1 ctx2 -> ctx1 = ctx2.
-
-Require Import Coq.Logic.Eqdep_dec.
-Require Import Coq.Arith.Peano_dec.
-
-Lemma snoc_eq : forall {A : Type} {n : nat} (l1 l2 : snoclist A n) (a : A),
-  l1 :: a = l2 :: a -> l1 = l2.
-Proof.
-intros A n l1 l2 a eq.
-inversion eq.
-apply inj_pair2_eq_dec in H0.
-- apply H0.
-- apply eq_nat_dec.
-Qed.
-
 (*
-Lemma snoclist_cong : forall {A : Type} {n m' : nat} (l : snoclist A n) (a : A)
-  (P Q : forall {m : nat}, snoclist A m -> snoclist A m'),
-  P l = Q l -> P (l :: a) = Q (l :: a).
+Consider: 
+unif_extra      only when !=Nil
+unif_perm_sigma ..
+unif_perm_const ..
+
+unif_taut sigma ty const:
+  sat_xi sigma (List.cons (ty, ty) const) ->
+  sat_xi sigma const
 *)
 
-Lemma subst_ctx_app : forall {n m : nat} (rul : s_rule) (ctx1 : context n) (ctx2 : context m),
-  subst1_ctx rul (ctx1 ++ ctx2) = subst1_ctx rul ctx1 ++ subst1_ctx rul ctx2.
+Inductive sat_xi : s_rules -> constraints -> Prop :=
+| unif_empty : sat_xi List.nil List.nil
+| unif_left (n : nat) (ty : type) sigma const :
+  sat_xi sigma const ->
+  sat_xi (List.cons (n, ty) sigma) (List.cons (TVar n, ty) const)
+| unif_right (n : nat) (ty : type) sigma const :
+  sat_xi sigma const ->
+  sat_xi (List.cons (n, ty) sigma) (List.cons (ty, TVar n) const)
+| unif_imp (tyl1 tyl2 tyr1 tyr2 : type) rul sigma const :
+  sat_xi (List.cons rul sigma) (List.cons (tyl2, tyr2) (List.cons (tyr1, tyl1) const)) ->
+  sat_xi (List.cons rul sigma) (List.cons (TImp tyl1 tyl2, TImp tyr1 tyr2) const)
+| unif_skip rul sigma const :
+  sat_xi sigma const -> sat_xi (List.cons rul sigma) const
+| unif_extra sigma eq const :
+  sat_xi sigma (List.cons eq const) -> sat_xi sigma const
+| unif_perm_sigma sigma1 sigma2 const :
+  sat_xi sigma1 const -> Permutation sigma1 sigma2 ->
+  sat_xi sigma2 const
+| unif_perm_const sigma const1 const2 :
+  sat_xi sigma const1 -> Permutation const1 const2 ->
+  sat_xi sigma const2.
+
+Lemma skipall_sat_xi : forall (sigma : s_rules), sat_xi sigma List.nil.
 Proof.
-intros n m rul ctx1 ctx2.
-induction ctx1.
-- simpl. induction ctx2.
-  + simpl.
-    rewrite comm_nil.
-    simpl. reflexivity.
-  + simpl.
-    rewrite ? comm_nilapp.
-    simpl. reflexivity.
-- simpl. induction ctx2.
-  + simpl in IHctx1. simpl.
-    rewrite ? comm_appnil.
-    simpl. rewrite IHctx1.
-    reflexivity.
-  + simpl.
-    rewrite ? comm_consapp_asso'.
-    simpl in IHctx1.
-    rewrite ? comm_consapp_asso in IHctx1.
-    assert (
-      subst1_ctx rul (snoclist_asso_1 ((ctx1 ++ ctx2) :: a0)) = 
-      snoclist_asso_1 (subst1_ctx rul ((ctx1 ++ ctx2) :: a0))
-    ) by apply subst_asso.
-    rewrite H in IHctx1. simpl in IHctx1.
-    assert (
-      subst1_ctx rul (ctx1 ++ ctx2) =
-      subst1_ctx rul ctx1 ++ subst1_ctx rul ctx2
-    ).
-    apply snoc_eq with (a := subst1_ty rul a0).
-    apply asso_eq. apply IHctx1.
-    simpl.
-    assert (
-      subst1_ctx rul (snoclist_asso_1 ((ctx1 :: a) ++ ctx2)) = 
-      snoclist_asso_1 (subst1_ctx rul ((ctx1 :: a) ++ ctx2))
-    ) by apply subst_asso.
-    rewrite H1.
-    assert (
-      subst1_ctx rul ((ctx1 :: a) ++ ctx2) =
-      (subst1_ctx rul ctx1 :: subst1_ty rul a) ++ subst1_ctx rul ctx2
-    ) by (apply IHctx2; apply H0).
-    rewrite H2. reflexivity.
+intro sigma. induction sigma.
+- apply unif_empty.
+- apply unif_skip. apply IHsigma.
 Qed.
 
-Lemma subst1_typed : forall {n : nat} (rul : s_rule) (ctx : context n) (pt : pterm n) (ty : type),
-  is_typed ctx pt ty -> is_typed (subst1_ctx rul ctx) pt (subst1_ty rul ty).
+Lemma appleft_sat_xi : forall (sigma : s_rules) (const1 const2 : constraints),
+  sat_xi sigma (List.app const1 const2) -> sat_xi sigma const1.
 Proof.
-intro n.
-intros rul ctx pt ty h.
-induction h.
-- simpl. apply typed_var.
-- simpl. apply typed_abs. simpl in IHh. apply IHh.
-- rewrite subst_ctx_app.
-  apply typed_app with (ty1 := subst1_ty rul ty1).
-  simpl in IHh1. apply IHh1. apply IHh2.
+induction const2.
+- rewrite List.app_nil_r. intro h. apply h.
+- intro h. apply IHconst2.
+  assert (Permutation (const1 ++ a :: const2)%list (a :: (const1 ++ const2))%list).
+  Check Permutation_cons_app.
+  apply (Permutation_sym (Permutation_cons_app
+    (l := (const1 ++ const2)) const1 const2 a
+    (Permutation_refl (const1 ++ const2)))).
+  assert (sat_xi sigma (a :: const1 ++ const2)%list).
+  apply (unif_perm_const sigma (const1 ++ a :: const2)%list (a :: (const1 ++ const2))%list).
+  apply h. apply H.
+  apply unif_extra with (eq := a).
+  apply H0.
 Qed.
 
-Lemma subst_typed : forall {n : nat} (sigma : s_rules) (ctx : context n) (pt : pterm n) (ty : type),
-  is_typed ctx pt ty -> is_typed (subst_ctx sigma ctx) pt (subst_ty sigma ty).
+Lemma appright_sat_xi : forall (sigma : s_rules) (const1 const2 : constraints),
+  sat_xi sigma (List.app const1 const2) -> sat_xi sigma const2.
 Proof.
-intros n sigma.
+induction const1.
+- simpl. intros const2 h. apply h.
+- intros const2 h. apply IHconst1.
+  simpl in h. apply unif_extra with (eq := a).
+  apply h.
+Qed.
+
+(* TODO *)
+Lemma nil_rules : forall (const : constraints) (ty1 ty2 : type),
+  sat_xi List.nil (List.cons (ty1, ty2) const) ->
+  ty1 <> ty2.
+Proof.
+intros const ty1 ty2 h.
+dependent induction h.
+- apply IHh with (const := const).
+Admitted.
+
+(* TODO *)
+Lemma subst_converge : forall (sigma : s_rules) (const : constraints) (ty1 ty2 : type),
+  sat_xi sigma ((ty1, ty2) :: const)%list ->
+  subst_ty sigma ty1 = subst_ty sigma ty2.
+Proof.
+intros sigma const ty1 ty2 h.
 induction sigma.
-- simpl. intros ctx pt ty h. apply h.
-- simpl. intros ctx pt ty h. apply IHsigma. apply subst1_typed. apply h.
+- dependent destruction h.
+  + simpl. admit.
+  + simpl. destruct sigma1.
+    * admit.
+    * apply Permutation_sym in H.
+      assert (~Permutation Datatypes.nil (s :: sigma1))
+        by (apply (Permutation_nil_cons (l := sigma1) (x := s))).
+      apply H0 in H. contradiction.
+  + simpl. destruct const1.
+    * admit.
+    * admit.
+- dependent destruction h.
+Admitted.
+
+(* Theorem *)
+
+Theorem bidir_typed_syn :
+  forall {n : nat} (gamma : context n) (st : sterm n) (ty : type) (const : constraints) (sigma : s_rules),
+  is_bidir_syn gamma st ty const ->
+  sat_xi sigma const ->
+  is_typed (subst_ctx sigma gamma) (strip_syn st) (subst_ty sigma ty)
+
+with bidir_typed_chk :
+  forall {n : nat} (gamma : context n) (ct : cterm n) (ty : type) (const : constraints) (sigma : s_rules),
+  is_bidir_chk gamma ct ty const ->
+  sat_xi sigma const ->
+  is_typed (subst_ctx sigma gamma) (strip_chk ct) (subst_ty sigma ty).
+
+Proof.
+- intros n gamma st ty const sigma hb hs.
+  induction hb.
+  + simpl.
+    rewrite dist_subst_ty.
+    apply (
+      typed_abs
+      (subst_ty sigma ty1) (subst_ctx sigma gamma)
+      (strip_syn st) (subst_ty sigma ty2)
+    ).
+    rewrite <- cons_subst_ctx.
+    apply IHhb. apply hs.
+  + simpl. apply bidir_typed_chk with (const := const).
+    apply H. apply hs.
+- intros n gamma ct ty const sigma hb hs.
+  induction hb.
+  + simpl.
+    rewrite single_subst_ctx.
+    apply (typed_var (subst_ty sigma ty)).
+  + simpl.
+    rewrite app_subst_ctx.
+    apply (
+      typed_app
+      (subst_ctx sigma gamma) (subst_ctx sigma delta)
+      (strip_chk ct1) (strip_syn st2)
+      (subst_ty sigma ty1) (subst_ty sigma ty2)
+    ).
+    * rewrite <- dist_subst_ty.
+      apply IHhb.
+      apply appleft_sat_xi with (const2 := const2).
+      apply hs.
+    * apply bidir_typed_syn with (const := const2).
+      apply H.
+      apply appright_sat_xi with (const1 := const1).
+      apply hs.
+  + simpl.
+    assert (subst_ty sigma ty1 = subst_ty sigma ty2).
+    apply subst_converge with (const := const).
+    apply hs.
+    rewrite <- H0.
+    apply bidir_typed_syn with (const := const).
+    apply H.
+    apply unif_extra with (eq := (ty1, ty2)).
+    apply hs.
 Qed.
+
+(* TODO: Principal Typing *)
 
 Definition is_princ : Type := forall {n : nat} (ctx : context n) (pt : pterm n) (ty : type),
   is_typed ctx pt ty -> forall (ctx' : context n) (ty' : type), is_typed ctx' pt ty' ->
   sig (fun (sigma : s_rules) => ctx' = subst_ctx sigma ctx /\ ty' = subst_ty sigma ty).
 
-(* ===== Labeled Terms ===== *)
-
-Inductive sterm : nat -> Type :=
-| SAbs {n} : sterm (S n) -> sterm n
-| SCir {n} : nat -> cterm n -> sterm n
-
-with cterm : nat -> Type :=
-| CVar : cterm 1
-| CApp {n} {m} : cterm n -> sterm m -> cterm (n + m)
-| CSqu {n} : sterm n -> cterm n.
-
-Inductive lterm : nat -> Type :=
-| LSyn {n} : sterm n -> lterm n
-| LChk {n} : cterm n -> lterm n.
-
-(* -- Strip -- *)
-
-Fixpoint strip_syn {n : nat} (t : sterm n) : pterm n :=
-match t with
-| SAbs t' => PAbs (strip_syn t')
-| SCir a t' => strip_chk t'
-end
-with strip_chk {n : nat} (t : cterm n) : pterm n :=
-match t with
-| CVar => PVar
-| CApp ct st => PApp (strip_chk ct) (strip_syn st)
-| CSqu t' => strip_syn t'
-end.
-
-Definition strip_labels {n : nat} (t : lterm n) : pterm n :=
-match t with
-| LSyn st => strip_syn st
-| LChk ct => strip_chk ct
-end.
-
-(* -- Label -- *)
-
-Fixpoint label_minus {n : nat} (t : pterm n) : sterm n :=
-match t with
-| PVar => SCir 0 CVar
-| PAbs t' => SAbs (label_minus t')
-| PApp t1 t2 => SCir 0 (CApp (CSqu (label_minus t1)) (label_minus t2))
-end.
-
-Fixpoint label_plus {n : nat} (t : pterm n) : cterm n :=
-match t with
-| PVar => CVar
-| PAbs t' => CSqu (SAbs (SCir 0 (label_plus t')))
-| PApp t1 t2 => CApp (label_plus t1) (SCir 0 (label_plus t2))
-end.
-
-Lemma label_strip_minus : forall {n : nat} (t : pterm n), strip_syn (label_minus t) = t.
-Proof.
-intros n t. induction t.
-- simpl. reflexivity.
-- simpl. rewrite IHt. reflexivity.
-- simpl. rewrite IHt1. rewrite IHt2. reflexivity.
-Qed.
-
-Lemma label_strip_plus : forall {n : nat} (t : pterm n), strip_chk (label_plus t) = t.
-Proof.
-intros n t. induction t.
-- simpl. reflexivity.
-- simpl. rewrite IHt. reflexivity.
-- simpl. rewrite IHt1. rewrite IHt2. reflexivity.
-Qed.
-
-Definition type_eq : Type := type * type.
-Definition constraints : Type := list type_eq.
-
-Inductive is_bidir_syn : forall {a : nat}, context a -> sterm a -> type -> constraints -> Prop :=
-| bidir_abs {n} ty1 gamma (st : sterm (S n)) ty2 const :
-  is_bidir_syn (gamma :: ty1) st ty2 const -> 
-  is_bidir_syn  gamma (SAbs st) (TImp ty1 ty2) const
-| bidir_cir {n} (a : nat) gamma (ct : cterm n) const :
-  is_bidir_chk gamma ct (TVar a) const ->
-  is_bidir_syn gamma (SCir a ct) (TVar a) const
-
-with is_bidir_chk : forall {a : nat}, context a -> cterm a -> type -> constraints -> Prop :=
-| bidir_var ty : is_bidir_chk [ty] CVar ty List.nil
-| bidir_app {n m} gamma delta (ct1 : cterm n) (st2 : sterm m) ty1 ty2 const1 const2 :
-  is_bidir_chk gamma ct1 (TImp ty1 ty2) const1 ->
-  is_bidir_syn delta st2 ty1 const2 ->
-  is_bidir_chk (gamma ++ delta) (CApp ct1 st2) ty2 (List.app const1 const2)
-| bidir_squ {n} gamma (st : sterm n) ty1 ty2 const :
-  is_bidir_syn gamma st ty1 const ->
-  is_bidir_chk gamma (CSqu st) ty2 (List.cons (ty1, ty2) const).
-
-Inductive is_bidir : forall {a : nat}, context a -> lterm a -> type -> constraints -> Prop :=
-| Sbidir {n} gamma (st : sterm n) ty const :
-  is_bidir_syn gamma st ty const ->
-  is_bidir gamma (LSyn st) ty const
-| Cbidir {n} gamma (ct : cterm n) ty const :
-  is_bidir_chk gamma ct ty const ->
-  is_bidir gamma (LChk ct) ty const.
-
-Inductive sat_const : s_rules -> constraints -> Prop :=
-| Unif_empty : sat_const List.nil List.nil.
-
-
-(*
-Lemma typed_lp : forall {a : nat} (ctx : context a) (lt : lterm a) (ty : type) (const : constraints),
-  is_bidir ctx lt ty const -> is_typed ctx (strip_labels lt) ty.
-Proof.
-intros a ctx lt ty const h.
-induction h.
-induction H.
-- Admitted.
-*)
-
-(* ===== Inference ===== *)
-
-
-
-
-
-
-(*
-Inductive b_synth : forall {a : nat} (newout : nat), context a -> pterm a -> type -> constraints -> Prop :=
-| syn_var (ctx : context 1) :
-  chk_test newout ctx PVar (S newout)
-| syn_test ty : b_synth  0 [ty] PVar ty List.nil
-
-with b_check : forall {a : nat} (newin : nat), context a -> pterm a -> type -> constraints -> Prop :=
-| chk_test ty : b_check 0 [ty] PVar ty List.nil.
-*)
-
-
-
-(*
-Fixpoint Bidir_synth {n : nat} (fresh : nat) (t : pterm n) : (nat * context n * type * constraints) :=
-match t in pterm n return (nat * context n * type * constraints) with
-| PAbs t' =>
-  let (temp, const) := Bidir_synth fresh t' in
-  let (temp', B) := temp in
-  let (fresh', ctx') := temp' in
-  match ctx' in snoclist _ (S n) return (nat * context n * type * constraints) with
-  | ctx'' :: A => (fresh', ctx'', TImp A B, const)
-  end
-| PVar =>
-  let (temp, const) := Bidir_check (S fresh) PVar (TVar fresh) in
-  let (fresh', ctx') := temp in
-  (fresh', ctx', (TVar fresh), const)
-| PApp pt1 pt2 =>
-  let (temp, const) := Bidir_check (S fresh) (PApp pt1 pt2) (TVar fresh) in
-  let (fresh', ctx') := temp in
-  (fresh', ctx', (TVar fresh), const)
-end
-
-with Bidir_check {n : nat} (fresh : nat) (t : pterm n) : type -> (nat * context n * constraints) :=
-fix Bidir_check fresh t ty :=
-match t in pterm n return (nat * context n * constraints) with
-| PVar => (fresh, [ty], List.nil)
-| PApp pt1 pt2 =>
-  let (temp, const2) := Bidir_synth fresh pt2 in
-  let (temp', A) := temp in
-  let (fresh', ctx2) := temp' in
-  let (temp, const1) := Bidir_check fresh' pt1 (TImp A ty) in
-  let (fresh'', ctx1) := temp' in
-  (fresh'', ctx1 ++ ctx2, List.app const1 const2)
-| PAbs t' =>
-  let (temp, const) := Bidir_synth fresh (PAbs t') in
-  let (temp', A) := temp in
-  let (fresh', ctx') := temp' in
-  (fresh', ctx', List.cons (A, ty) const)
-end.
-
-*)
 
 
 
