LabeledLambda.v
@@ -1,0 +1,68 @@
+Require Import PlanarLambda.
+
+(* ===== Labeled Terms ===== *)
+
+Inductive sterm : nat -> Type :=
+| SAbs {n} : sterm (S n) -> sterm n
+| SCir {n} : nat -> cterm n -> sterm n
+
+with cterm : nat -> Type :=
+| CVar : cterm 1
+| CApp {n} {m} : cterm n -> sterm m -> cterm (n + m)
+| CSqu {n} : sterm n -> cterm n.
+
+Inductive lterm : nat -> Type :=
+| LSyn {n} : sterm n -> lterm n
+| LChk {n} : cterm n -> lterm n.
+
+(* -- Strip -- *)
+
+Fixpoint strip_syn {n : nat} (t : sterm n) : pterm n :=
+match t with
+| SAbs t' => PAbs (strip_syn t')
+| SCir a t' => strip_chk t'
+end
+with strip_chk {n : nat} (t : cterm n) : pterm n :=
+match t with
+| CVar => PVar
+| CApp ct st => PApp (strip_chk ct) (strip_syn st)
+| CSqu t' => strip_syn t'
+end.
+
+Definition strip_labels {n : nat} (t : lterm n) : pterm n :=
+match t with
+| LSyn st => strip_syn st
+| LChk ct => strip_chk ct
+end.
+
+(* -- Label -- *)
+
+Fixpoint label_minus {n : nat} (t : pterm n) : sterm n :=
+match t with
+| PVar => SCir 0 CVar
+| PAbs t' => SAbs (label_minus t')
+| PApp t1 t2 => SCir 0 (CApp (CSqu (label_minus t1)) (label_minus t2))
+end.
+
+Fixpoint label_plus {n : nat} (t : pterm n) : cterm n :=
+match t with
+| PVar => CVar
+| PAbs t' => CSqu (SAbs (SCir 0 (label_plus t')))
+| PApp t1 t2 => CApp (label_plus t1) (SCir 0 (label_plus t2))
+end.
+
+Lemma label_strip_minus : forall {n : nat} (t : pterm n), strip_syn (label_minus t) = t.
+Proof.
+intros n t. induction t.
+- simpl. reflexivity.
+- simpl. rewrite IHt. reflexivity.
+- simpl. rewrite IHt1. rewrite IHt2. reflexivity.
+Qed.
+
+Lemma label_strip_plus : forall {n : nat} (t : pterm n), strip_chk (label_plus t) = t.
+Proof.
+intros n t. induction t.
+- simpl. reflexivity.
+- simpl. rewrite IHt. reflexivity.
+- simpl. rewrite IHt1. rewrite IHt2. reflexivity.
+Qed.
