Subst.v
@@ -1,0 +1,157 @@
+Require Import Nat.
+Require Import Snoclist.
+Import SnoclistNotations.
+Require Import PlanarLambda.
+Require Import Types.
+
+Require Import Coq.Program.Equality.
+Require Import Arith.
+Require List.
+
+Definition s_rule : Type := nat * type.
+Definition s_rules : Type := list s_rule.
+
+Fixpoint subst1_ty (rul : s_rule) (ty : type) : type :=
+match ty with
+| TVar n => let (m, u) := rul in
+  match eqb n m with
+  | true => u
+  | false => ty
+  end
+| TImp ty1 ty2 => TImp (subst1_ty rul ty1) (subst1_ty rul ty2)
+end.
+
+Fixpoint subst_ty (sigma : s_rules) (ty : type) : type :=
+match sigma with
+| List.nil => ty
+| List.cons rul sigma' =>
+  subst_ty sigma' (subst1_ty rul ty)
+end.
+
+Fixpoint subst1_ctx (rul : s_rule) {n : nat} (ctx : context n) : context n :=
+match ctx with
+| [] => []
+| ctx' :: ty => (subst1_ctx rul ctx') :: (subst1_ty rul ty)
+end.
+
+Fixpoint subst_ctx (sigma : s_rules) {n : nat} (ctx : context n) : context n :=
+match sigma with
+| List.nil => ctx
+| List.cons rul sigma' =>
+  subst_ctx sigma' (subst1_ctx rul ctx)
+end.
+
+(* Lemmas *)
+
+Lemma subst_asso : forall {m n : nat} (rul : s_rule) (ctx : context (S m + n)),
+  subst1_ctx rul (snoclist_asso_1 ctx) = 
+  snoclist_asso_1 (subst1_ctx rul ctx).
+Proof. intros m n rul ctx. apply P_asso. Qed.
+
+Lemma subst_ctx_app : forall {n m : nat} (rul : s_rule) (ctx1 : context n) (ctx2 : context m),
+  subst1_ctx rul (ctx1 ++ ctx2) = subst1_ctx rul ctx1 ++ subst1_ctx rul ctx2.
+Proof.
+intros n m rul ctx1 ctx2.
+induction ctx1.
+- simpl. induction ctx2.
+  + simpl.
+    rewrite comm_nil.
+    simpl. reflexivity.
+  + simpl.
+    rewrite ? comm_nilapp.
+    simpl. reflexivity.
+- simpl. induction ctx2.
+  + simpl in IHctx1. simpl.
+    rewrite ? comm_appnil.
+    simpl. rewrite IHctx1.
+    reflexivity.
+  + simpl.
+    rewrite ? comm_consapp_asso'.
+    simpl in IHctx1.
+    rewrite ? comm_consapp_asso in IHctx1.
+    assert (
+      subst1_ctx rul (snoclist_asso_1 ((ctx1 ++ ctx2) :: a0)) = 
+      snoclist_asso_1 (subst1_ctx rul ((ctx1 ++ ctx2) :: a0))
+    ) by apply subst_asso.
+    rewrite H in IHctx1. simpl in IHctx1.
+    assert (
+      subst1_ctx rul (ctx1 ++ ctx2) =
+      subst1_ctx rul ctx1 ++ subst1_ctx rul ctx2
+    ).
+    apply snoc_eq with (a := subst1_ty rul a0).
+    apply asso_eq. apply IHctx1.
+    simpl.
+    assert (
+      subst1_ctx rul (snoclist_asso_1 ((ctx1 :: a) ++ ctx2)) = 
+      snoclist_asso_1 (subst1_ctx rul ((ctx1 :: a) ++ ctx2))
+    ) by apply subst_asso.
+    rewrite H1.
+    assert (
+      subst1_ctx rul ((ctx1 :: a) ++ ctx2) =
+      (subst1_ctx rul ctx1 :: subst1_ty rul a) ++ subst1_ctx rul ctx2
+    ) by (apply IHctx2; apply H0).
+    rewrite H2. reflexivity.
+Qed.
+
+Lemma dist_subst1_ty : forall (rul : s_rule) (ty1 ty2 : type),
+  subst1_ty rul (TImp ty1 ty2) = TImp (subst1_ty rul ty1) (subst1_ty rul ty2).
+Proof. simpl. reflexivity. Qed.
+
+Lemma dist_subst_ty : forall (sigma : s_rules) (ty1 ty2 : type),
+  subst_ty sigma (TImp ty1 ty2) = TImp (subst_ty sigma ty1) (subst_ty sigma ty2).
+Proof.
+intro sigma. induction sigma.
+- simpl. reflexivity.
+- simpl. intros. apply IHsigma.
+Qed.
+
+Lemma cons_subst_ctx : forall {n : nat} (sigma : s_rules) (gamma : context n) (ty : type),
+  subst_ctx sigma (gamma :: ty) =
+  subst_ctx sigma gamma :: subst_ty sigma ty.
+Proof.
+intros n sigma. induction sigma.
+- simpl. reflexivity.
+- simpl. intros gamma ty. apply IHsigma.
+Qed.
+
+Lemma single_subst_ctx : forall (sigma : s_rules) (ty : type),
+  subst_ctx sigma [ty] = [subst_ty sigma ty].
+Proof.
+intro sigma. induction sigma.
+- simpl. reflexivity.
+- simpl. intros ty. apply IHsigma.
+Qed.
+
+Lemma app_subst_ctx : forall {m n : nat} (sigma : s_rules) (ctx1 : context n) (ctx2 : context m),
+  subst_ctx sigma (ctx1 ++ ctx2) = subst_ctx sigma ctx1 ++ subst_ctx sigma ctx2.
+Proof.
+intros m n sigma. induction sigma.
+- simpl. reflexivity.
+- simpl. intros ctx1 ctx2.
+  rewrite subst_ctx_app.
+  apply IHsigma.
+Qed.
+
+(* Typing *)
+
+Lemma subst1_typed : forall {n : nat} (rul : s_rule) (ctx : context n) (pt : pterm n) (ty : type),
+  is_typed ctx pt ty -> is_typed (subst1_ctx rul ctx) pt (subst1_ty rul ty).
+Proof.
+intro n.
+intros rul ctx pt ty h.
+induction h.
+- simpl. apply typed_var.
+- simpl. apply typed_abs. simpl in IHh. apply IHh.
+- rewrite subst_ctx_app.
+  apply typed_app with (ty1 := subst1_ty rul ty1).
+  simpl in IHh1. apply IHh1. apply IHh2.
+Qed.
+
+Lemma subst_typed : forall {n : nat} (sigma : s_rules) (ctx : context n) (pt : pterm n) (ty : type),
+  is_typed ctx pt ty -> is_typed (subst_ctx sigma ctx) pt (subst_ty sigma ty).
+Proof.
+intros n sigma.
+induction sigma.
+- simpl. intros ctx pt ty h. apply h.
+- simpl. intros ctx pt ty h. apply IHsigma. apply subst1_typed. apply h.
+Qed.
